sorting-algorithms/SortSpec.v
@@ -1,17 +1,53 @@
 Require Import Coq.Lists.List.
-Require Import Permutation.
+Require Import Coq.Sorting.Permutation.
+Require Import Omega.
 
 Notation "[ ]" := nil.
 Notation "[ x ; .. ; y ]" := (cons x .. (cons y nil) ..).
 
 (** A sorted list should be arranged in increasing order. *)
 Inductive Sorted : list nat -> Prop :=
-| Sorted_Nil : Sorted []
-| Sorted_Singleton : forall x, Sorted [x]
-| Sorted_Cons : forall x y l, x <= y /\ Sorted (y :: l) -> Sorted (x :: y :: l).
+| Sorted_nil : Sorted []
+| Sorted_singleton : forall x,
+    Sorted [x]
+| Sorted_cons : forall x y l,
+    x <= y /\ Sorted (y :: l) -> Sorted (x :: y :: l).
 
-(** A sorting algorithm should make the list sorted, and keep permutation. *)
-Definition SortSpec (sort : list nat -> list nat) :=
-  forall (l : list nat), Sorted (sort l) /\ Permutation l (sort l).
+Inductive StronglySorted : list nat -> Prop :=
+| SSorted_nil : StronglySorted []
+| SSorted_cons : forall x l,
+    StronglySorted l -> Forall (fun y => x <= y) l -> StronglySorted (x :: l).
 
 Hint Constructors Sorted.
+
+Theorem sorted_equivalent : forall (l : list nat),
+  Sorted l <-> StronglySorted l.
+Proof.
+  Ltac solver :=
+    match goal with
+    | [ H : and ?P ?Q |- _ ] => destruct H
+    | [ H : Sorted (_ :: _ :: _) |- _ ] => inversion H; subst; clear H
+    | [ H : Sorted (_ :: nil) |- _ ] => clear H
+    | [ H : StronglySorted (_ :: _) |- _ ] => inversion H; subst; clear H
+    | [ H : Forall _ (_ :: _) |- _ ] => inversion H; clear H
+    | [ |- Sorted _ ] => constructor
+    | [ |- StronglySorted _ ] => constructor
+    end; auto; intuition.
+  split; induction l; intros; repeat solver.
+  - destruct l; repeat solver.
+  - destruct l; repeat solver.
+    constructor; auto.
+    apply Forall_impl with (P := (fun y : nat => n <= y)); auto.
+    intros; omega.
+  - destruct l; repeat solver.
+Qed.
+
+Module Type Sorting.
+
+Parameter sort : list nat -> list nat.
+
+(** A sorting algorithm should make the list sorted, and keep permutation. *)
+Axiom sort_algorithm : forall (l : list nat),
+  Sorted (sort l) /\ Permutation l (sort l).
+
+End Sorting.
